src/program_proof/alloc/alloc_proof.v
@@ -2,6 +2,8 @@ From Perennial.program_proof Require Import proof_prelude.
 From Perennial.program_proof Require Import util_proof.
 From Goose.github_com.mit_pdos.goose_nfsd Require Import alloc.
 
+(* TODO: this file isn't using typed_slice, should fix that *)
+
 Section proof.
 Context `{!heapG Σ}.
 
@@ -56,6 +58,100 @@ Proof.
   subst max; word.
 Qed.
 
+Lemma bits_lookup_byte (max: u64) (bits: list u8) (num: u64) :
+  int.Z max = 8 * length bits →
+  int.Z num < int.Z max →
+  ∃ (b:u8), (b2val <$> bits) !! int.nat (word.divu num 8) = Some (b2val b).
+Proof.
+  intros Hmax Hnum.
+  assert (int.Z num / 8 < length bits).
+  { apply Zdiv_lt_upper_bound; lia. }
+  destruct (list_lookup_lt _ bits (Z.to_nat (int.Z num / 8)%Z)) as [b Hlookup].
+  { apply Nat2Z.inj_lt.
+    word. }
+  exists b.
+  rewrite list_lookup_fmap.
+  apply fmap_Some.
+  eexists; split; eauto.
+  rewrite word.unsigned_divu_nowrap; auto.
+Qed.
+
+(* TODO: identical to freeBit proof, would be nice to share some of this *)
+Lemma wp_MarkUsed max l (bn: u64) :
+  int.Z bn < int.Z max →
+  {{{ is_alloc max l }}}
+    Alloc__MarkUsed #l #bn
+  {{{ RET #(); True }}}.
+Proof.
+  intros Hbound.
+  iIntros (Φ) "H HΦ". iNamed "H".
+  wp_call.
+  wp_loadField.
+  wp_apply (acquire_spec with "[$]").
+  iIntros "[Hlocked Hlinv]".
+  wp_pures.
+  iNamed "Hlinv".
+  wp_loadField.
+  destruct (bits_lookup_byte max bits bn) as [b Hlookup]; [ done | done | ].
+  wp_apply (wp_SliceGet with "[$Hbits]"); first by eauto.
+  iIntros "[Hbits _]".
+  wp_loadField.
+  wp_apply (wp_SliceSet with "[$Hbits]").
+  { iSplit; iPureIntro; auto.
+    rewrite Hlookup; eauto. }
+  iIntros "Hbits".
+  wp_pures.
+  wp_loadField.
+  wp_apply (release_spec with "[$His_lock $Hlocked next bitmap Hbits]").
+  { rewrite -list_fmap_insert.
+    iExists _, _, _; iFrame "∗%".
+    rewrite insert_length.
+    iFrame "%". }
+  by iApply "HΦ".
+Qed.
+
+Local Ltac Zify.zify_post_hook ::= Z.div_mod_to_equations.
+
+Lemma wp_MkMaxAlloc (max: u64) :
+  0 < int.Z max →
+  int.Z max `mod` 8 = 0 →
+  {{{ True }}}
+    MkMaxAlloc #max
+  {{{ l, RET #l; is_alloc max l }}}.
+Proof.
+  iIntros (Hbound Hmod Φ) "_ HΦ".
+  wp_call.
+  rewrite -> bool_decide_eq_true_2 by word.
+  wp_pures.
+  rewrite bool_decide_eq_true_2; last first.
+  { repeat (f_equal; try word). }
+  wp_pures.
+  wp_apply wp_new_slice; first by auto.
+  iIntros (bitmap_s) "Hs".
+  wp_pures.
+  iApply is_slice_to_small in "Hs".
+  replace (replicate (int.nat (word.divu max 8)) (zero_val byteT))
+          with (b2val <$> replicate (int.nat (word.divu max 8)) (U8 0));
+    last first.
+  { rewrite fmap_replicate //. }
+  wp_apply (wp_MkAlloc with "[$Hs]").
+  { rewrite replicate_length.
+    word. }
+  { rewrite replicate_length.
+    word. }
+  iIntros (a_l) "#Ha".
+  rewrite replicate_length.
+  wp_pures.
+  wp_apply (wp_MarkUsed with "Ha").
+  { word. }
+  wp_pures.
+  iModIntro.
+  iApply "HΦ".
+  iExactEq "Ha".
+  f_equal.
+  word.
+Qed.
+
 (* TODO: this is false as written, but the idea is to define a wrapper around
    MkAlloc that does satisfy this spec *)
 Lemma wp_MkAlloc' (max: u64) :
@@ -104,24 +200,6 @@ Proof.
       iFrame "∗%".
       iPureIntro.
       revert Heqb; word.
-Qed.
-
-Lemma bits_lookup_byte (max: u64) (bits: list u8) (num: u64) :
-  int.Z max = 8 * length bits →
-  int.Z num < int.Z max →
-  ∃ (b:u8), (b2val <$> bits) !! int.nat (word.divu num 8) = Some (b2val b).
-Proof.
-  intros Hmax Hnum.
-  assert (int.Z num / 8 < length bits).
-  { apply Zdiv_lt_upper_bound; lia. }
-  destruct (list_lookup_lt _ bits (Z.to_nat (int.Z num / 8)%Z)) as [b Hlookup].
-  { apply Nat2Z.inj_lt.
-    word. }
-  exists b.
-  rewrite list_lookup_fmap.
-  apply fmap_Some.
-  eexists; split; eauto.
-  rewrite word.unsigned_divu_nowrap; auto.
 Qed.
 
 Lemma wp_allocBit (max: u64) (l: loc) :
@@ -235,40 +313,6 @@ Proof.
   by iApply "HΦ".
 Qed.
 
-(* TODO: identical to freeBit proof, would be nice to share some of this *)
-Lemma wp_MarkUsed max l (bn: u64) :
-  int.Z bn < int.Z max →
-  {{{ is_alloc max l }}}
-    Alloc__MarkUsed #l #bn
-  {{{ RET #(); True }}}.
-Proof.
-  intros Hbound.
-  iIntros (Φ) "H HΦ". iNamed "H".
-  wp_call.
-  wp_loadField.
-  wp_apply (acquire_spec with "[$]").
-  iIntros "[Hlocked Hlinv]".
-  wp_pures.
-  iNamed "Hlinv".
-  wp_loadField.
-  destruct (bits_lookup_byte max bits bn) as [b Hlookup]; [ done | done | ].
-  wp_apply (wp_SliceGet with "[$Hbits]"); first by eauto.
-  iIntros "[Hbits _]".
-  wp_loadField.
-  wp_apply (wp_SliceSet with "[$Hbits]").
-  { iSplit; iPureIntro; auto.
-    rewrite Hlookup; eauto. }
-  iIntros "Hbits".
-  wp_pures.
-  wp_loadField.
-  wp_apply (release_spec with "[$His_lock $Hlocked next bitmap Hbits]").
-  { rewrite -list_fmap_insert.
-    iExists _, _, _; iFrame "∗%".
-    rewrite insert_length.
-    iFrame "%". }
-  by iApply "HΦ".
-Qed.
-
 Lemma wp_AllocNum max l :
   {{{ is_alloc max l }}}
     Alloc__allocBit #l
@@ -296,3 +340,5 @@ Proof.
 Qed.
 
 End proof.
+
+Ltac Zify.zify_post_hook ::= idtac.
